lean/VerifiedFipsCryptography/Specs/SHA1.lean
@@ -28,12 +28,70 @@ def ROTL (n : Nat) (x : Word) : Word :=
   let nn : UInt32 := n.toUInt32
   ((x <<< nn) ||| (x >>> (32 - nn)))
 
--- Padding function
+/-
+This is not ideal, but given how Aeneas generates the looping code in `algorithms.sha1.pad_message_loop`,
+it's incredibly difficult to untangle the reasoning and show equivalence to the pure FP implementation.
+-/
+def padMessageLoop (ml : UInt64) (paddedMsg : Array UInt8) (zeroPaddingLength : ℕ) (i : ℕ) : Array UInt8 :=
+  if i < zeroPaddingLength then
+    let paddedMsg1 := paddedMsg.push 0
+    let i1 := i + 1
+    padMessageLoop ml paddedMsg1 zeroPaddingLength i1
+  else
+    let lengthBytes := Array.mkArray 8 (0 : UInt8)
+    let i1 := ml >>> 56
+    let i2 := UInt64.toUInt8 (i1 &&& 255)
+    let i3 := ml >>> 48
+    let lengthBytes1 := lengthBytes.set (0 : Fin 8) i2
+    let i4 := UInt64.toUInt8 (i3 &&& 255)
+    let i5 := ml >>> 40
+    let lengthBytes2 := lengthBytes1.set (1 : Fin 8) i4
+    let i6 := UInt64.toUInt8 (i5 &&& 255)
+    let i7 := ml >>> 32
+    let lengthBytes3 := lengthBytes2.set (2 : Fin 8) i6
+    let i8 := UInt64.toUInt8 (i7 &&& 255)
+    let i9 := ml >>> 24
+    let lengthBytes4 := lengthBytes3.set (3 : Fin 8) i8
+    let i10 := UInt64.toUInt8 (i9 &&& 255)
+    let i11 := ml >>> 16
+    let lengthBytes5 := lengthBytes4.set (4 : Fin 8) i10
+    let i12 := UInt64.toUInt8 (i11 &&& 255)
+    let i13 := ml >>> 8
+    let lengthBytes6 := lengthBytes5.set (5 : Fin 8) i12
+    let i14 := UInt64.toUInt8 (i13 &&& 255)
+    let i15 := ml >>> 0
+    let lengthBytes7 := lengthBytes6.set (6 : Fin 8) i14
+    let i16 := UInt64.toUInt8 (i15 &&& 255)
+    let lengthBytes8 := lengthBytes7.set (7 : Fin 8) i16
+    paddedMsg ++ lengthBytes8
+
+/-
+We use this one when showing equivalence.
+The natural next step would be to show equivalence to `padMessage'` (the old FP version)
+and thus derive the full equivalence transitively. Not sure how hard that would be,
+but working purely in Lean types definitely makes it easier.
+-/
 def padMessage (msg : ByteArray) : ByteArray :=
+  -- Step 1: Compute message length in bits
   let ml := UInt64.ofNat (msg.size * 8) -- Message length in bits
-  let padding : ByteArray := ByteArray.mk #[0x80] -- Append '1' bit and seven '0' bits
+  -- Step 2: Append the padding bit (0x80)
+  let padding : ByteArray := ByteArray.mk #[0x80]
+  -- Step 3: Calculate zero-padding length
   let zeroPaddingLength := (56 - ((msg.size + 1) % 64)) % 64
+  -- Step 4: Append zero padding
+  ⟨padMessageLoop ml (msg ++ padding).1 zeroPaddingLength 0⟩
+
+-- Padding function
+def padMessage' (msg : ByteArray) : ByteArray :=
+  -- Step 1: Compute message length in bits
+  let ml := UInt64.ofNat (msg.size * 8) -- Message length in bits
+  -- Step 2: Append the padding bit (0x80)
+  let padding : ByteArray := ByteArray.mk #[0x80]
+  -- Step 3: Calculate zero-padding length
+  let zeroPaddingLength := (56 - ((msg.size + 1) % 64)) % 64
+  -- Step 4: Append zero padding
   let zeroPadding := ByteArray.mk (List.replicate zeroPaddingLength 0).toArray
+  -- Step 5: Append message length as 64-bit big-endian integer
   let lengthBytes := ByteArray.mk $ ((List.range 8).reverse.map fun (i: Nat) =>
     ((ml >>> (i * 8).toUInt64) &&& 0xFF).toUInt8).toArray
   msg ++ padding ++ zeroPadding ++ lengthBytes
@@ -49,6 +107,37 @@ def chunkify (msg : ByteArray) : Array ByteArray :=
 -- Convert a 4-byte slice to a Word (UInt32)
 def bytesToWord (bytes : ByteArray) : Word :=
   bytes.foldl (fun acc b => (acc <<< 8) ||| b.toUInt32) 0
+
+def hashToVecLoop (finalHash : Vector Word 5) (resultBytes : Array UInt8) (index : ℕ) : Array UInt8 :=
+  if h : index < 5 then
+    let word := finalHash[index]
+    let i1 := word >>> 24
+    let i2 := UInt32.toUInt8 (i1 &&& 255)
+    let resultBytes1 := resultBytes.push i2
+    let i3 := word >>> 16
+    let i4 := UInt32.toUInt8 (i3 &&& 255)
+    let resultBytes2 := resultBytes1.push i4
+    let i5 := word >>> 8
+    let i6 := UInt32.toUInt8 (i5 &&& 255)
+    let resultBytes3 := resultBytes2.push i6
+    let i7 := word >>> 0
+    let i8 := UInt32.toUInt8 (i7 &&& 255)
+    let resultBytes4 := resultBytes3.push i8
+    let index1 := index + 1
+    hashToVecLoop finalHash resultBytes4 index1
+  else
+    resultBytes
+
+def hashToVec (finalHash : Vector Word 5) : ByteArray :=
+  ⟨hashToVecLoop finalHash #[] 0⟩
+
+-- Replace again.
+-- def hashToVec (finalHash : Vector Word 5) : ByteArray :=
+--   finalHash.toList.foldl (init := ByteArray.empty) fun acc (h: Word) =>
+--     let tmp := (List.range 4).toArray.reverse.map
+--       (fun (i: Nat) => ((h >>> (i.toUInt32 * 8)) &&& 0xFF).toUInt8)
+--       |> ByteArray.mk
+--     acc ++ tmp
 
 -- Main hash function
 def hash (message : ByteArray) : ByteArray :=
@@ -91,12 +180,7 @@ def hash (message : ByteArray) : ByteArray :=
     return ⟨h0.toList.zipWith (· + ·) [a, b, c, d, e], by simp⟩
 
   -- Concatenate the final hash values into a ByteArray
-  let resultBytes := finalHash.toList.foldl (init := ByteArray.empty) fun acc (h: Word) =>
-    let tmp := (List.range 4).toArray.reverse.map
-      (fun (i: Nat) => ((h >>> (i.toUInt32 * 8)) &&& 0xFF).toUInt8)
-      |> ByteArray.mk
-    acc ++ tmp
-  resultBytes
+  hashToVec finalHash
 
 end SHA1
 
